Merge Translate, Morphisms, Fix

theories/Interp/Interp.v
@@ -1,26 +1,88 @@
+(** An event morphism [E ~> F] lifts to an itree morphism [itree E ~> itree F]
+    by mapping the event morphism across each visible event.  We call this
+    process _event translation_.
+
+
+    Translate is defined separately from the itree Morphisms because it is
+    conceptually at a different level: translation always yields strong
+    bisimulations.  We can relate translation and interpretation via the law:
+
+    translate h t ≈ interp (liftE ∘ h) t
+*)
+
+(** The semantics of an interaction tree [itree E ~> M] can be
+    derived from semantics given for every individual effect
+    [E ~> M].
+
+    We define the following terminology for this library.
+    Other sources may have different usages for the same or related
+    words.
+
+    The notation [E ~> F] means [forall T, E T -> F T]
+    (in [ITree.Basics]).
+    It can mean many things, including the following.
+
+    - The semantics of itrees are given as monad morphisms
+      [itree E ~> M], also called "interpreters".
+
+    - "Itree interpreters" (or "itree morphisms") are monad morphisms
+      [itree E ~> itree F]. Most interpreters in this library are
+      actually itree interpreters.
+
+    This module provides various ways of defining interpreters
+    from effect handlers and other similar structures.
+
+    - "Effect handlers" are functions [E ~> M] where [M] is a monad.
+
+    - "Itree effect handlers" are functions [E ~> itree F].
+
+    Categorically, this boils down to saying that [itree] is a free
+    monad (not quite, but close enough).
+ *)
+
+(* begin hide *)
+From ITree Require Import
+     Basics.Basics
+     Core.ITree
+     Indexed.Sum.
+
+Import ITree.Basics.Basics.Monads.
+Import ITreeNotations.
+
+Open Scope itree_scope.
+(* end hide *)
+
+(** A plain effect morphism [E ~> F] defines an itree morphism
+    [itree E ~> itree F]. *)
+Definition translateF {E F R} (h : E ~> F) (rec: itree E R -> itree F R) (t : itreeF E R _) : itree F R  :=
+  match t with
+  | RetF x => Ret x
+  | TauF t => Tau (rec t)
+  | VisF e k => Vis (h _ e) (fun x => rec (k x))
+  end.
+
+CoFixpoint translate {E F R} (h : E ~> F) (t : itree E R) : itree F R
+  := translateF h (translate h) (observe t).
+
+(** An itree effect handler [E ~> itree F] defines an
+    itree morphism [itree E ~> itree F]. *)
+Definition interp {E F : Type -> Type} (h : E ~> itree F) :
+  itree E ~> itree F := fun R =>
+  ITree.aloop (fun t =>
+    match observe t with
+    | RetF r => inr r
+    | TauF t => inl (Ret t)
+    | VisF e k => inl (ITree.map k (h _ e))
+    end).
+(* TODO: this does a map, and aloop does a bind. We could fuse those
+   by giving aloop a continuation to compose its bind with.
+   (coyoneda...) *)
 (* Implementation of the fixpoint combinator over interaction
  * trees.
  *
  * The implementation is based on the discussion here
  *   https://gmalecha.github.io/reflections/2018/compositional-coinductive-recursion-in-coq
  *)
-
-Require Import Paco.paco.
-
-From Coq Require Import
-     Program
-     Lia
-     Setoid
-     Morphisms
-     RelationClasses.
-
-From ITree Require Import
-     Basics.Basics
-     Core.ITree
-     Interp.Morphisms
-     Indexed.Sum.
-
-Import ITreeNotations.
 
 (* The indexed type [D : Type -> Type] gives the signature of
    a set of functions. For example, a pair of mutually recursive
