theories/Effects/Env.v
@@ -16,7 +16,8 @@ From ITree Require Import
      Core.ITree
      Indexed.Sum
      Indexed.OpenSum
-     Interp.Morphisms.
+     Interp.Interp
+     Effects.State.
 
 Import ITree.Basics.Basics.Monads.
 
