theories/Effects/State.v
@@ -1,0 +1,148 @@
+(* begin hide *)
+From ExtLib Require Import
+     Structures.Monoid.
+
+From ITree Require Import
+     Basics.Basics
+     Core.ITree
+     Indexed.Sum
+     Interp.Interp.
+
+Import ITree.Basics.Basics.Monads.
+Import ITreeNotations.
+
+Open Scope itree_scope.
+(* end hide *)
+
+(* Stateful handlers [E ~> stateT S (itree F)] and morphisms
+   [E ~> state S] define stateful itree morphisms
+   [itree E ~> stateT S (itree F)]. *)
+
+Definition interp_state {E F S} (h : E ~> stateT S (itree F)) :
+  itree E ~> stateT S (itree F) :=
+  fun R t0 s0 =>
+    ITree.aloop (fun st =>
+      let s := fst st in let t := snd st in
+      match t.(observe) with
+      | RetF r => inr (s, r)
+      | TauF t => inl (Ret (s, t))
+      | VisF e k => inl (ITree.map (fun '(s, x) => (s, k x)) (h _ e s))
+      end) (s0, t0).
+
+(** The "reader" and "writer" variants are specializations
+    of the above stateful morphisms when the state cannot
+    be changed or read (i.e., append only). *)
+
+Definition interp_reader {E F R} (h : R -> E ~> itree F) :
+  R -> itree E ~> itree F :=
+  fun r => interp (h r).
+
+Definition translate_reader {E F R} (h : R -> E ~> identity) :
+  R -> itree E ~> itree F :=
+  fun r => interp (fun _ e => Ret (h r _ e)).
+
+Definition map_fst {A A' B} (f : A -> A') : A * B -> A' * B :=
+  fun '(a, b) => (f a, b).
+
+Definition interp_writer {E F W} {Monoid_W : Monoid W} (h : E ~> writerT W (itree F)) :
+  itree E ~> writerT W (itree F) :=
+  fun _ t =>
+    interp_state
+      (fun _ e s => ITree.map (map_fst (monoid_plus Monoid_W s)) (h _ e))
+      _ t (monoid_unit Monoid_W).
+
+(* todo(gmm): this can be stronger if we allow for a `can_returnE` *)
+Inductive can_return {E : Type -> Type} {t : Type} : itree E t -> t -> Prop :=
+| can_return_Ret {x} : can_return (Ret x) x
+| can_return_Tau {tr x} (_ : can_return tr x) : can_return (Tau tr) x
+| can_return_Vis {u e k} {x: u} {res} (_ : can_return (k x) res)
+  : can_return (Vis e k) res.
+
+(** A propositional "interpreter"
+    This can be useful for non-determinism.
+ *)
+Section interp_prop.
+  Context {E F : Type -> Type}.
+
+  Definition eff_hom_prop : Type :=
+    forall t, E t -> itree F t -> Prop.
+
+  CoInductive interp_prop (f : eff_hom_prop) (R : Type)
+  : itree E R -> itree F R -> Prop :=
+  | ipRet : forall x, interp_prop f R (Ret x) (Ret x)
+  | ipVis : forall {T} {e : E T} {e' : itree F T}
+              (k : _ -> itree E R) (k' : T -> itree F R),
+      f _ e e' ->
+      (forall x,
+          can_return e' x ->
+          interp_prop f R (k x) (k' x)) ->
+      interp_prop f R (Vis e k) (ITree.bind e' k')
+  | ipDelay : forall a b, interp_prop f R a b ->
+                     interp_prop f R (Tau a) (Tau b).
+
+End interp_prop.
+Arguments eff_hom_prop _ _ : clear implicits.
+
+(** An extensional stateful handler *)
+Section eff_hom_e.
+  Context {E F : Type -> Type}.
+
+  (* note(gmm): you should be able to add effects here
+   * using a monad transformer. In that case, the type
+   * of `eval` is:
+   *
+   *   forall t, E t -> m (itree F) (t * eff_hom_e)
+   *
+   * but you have the usual conditions on strictly positive uses
+   *)
+  CoInductive eff_hom_e : Type :=
+  { eval : forall t, E t -> itree F (eff_hom_e * t) }.
+
+  Definition interp_e (h : eff_hom_e) : itree E ~> itree F := fun R t =>
+    ITree.aloop (fun '(s, t) =>
+      match t.(observe) with
+      | RetF r => inr r
+      | TauF t => inl (Ret (s, t))
+      | VisF e k => inl (ITree.map (fun '(s, x) => (s, k x)) (h.(eval) _ e))
+      end) (h, t).
+
+End eff_hom_e.
+
+Section into.
+  Context {E F : Type -> Type}.
+
+  Definition into (h : E ~> itree F) : (E +' F) ~> itree F :=
+    fun _ e =>
+      match e with
+      | inl1 e => h _ e
+      | inr1 e => ITree.liftE e
+      end.
+
+  Definition into_state {s} (h : E ~> stateT s (itree F)) :
+    (E +' F) ~> stateT s (itree F) :=
+    fun _ e s =>
+      match e with
+      | inl1 e => h _ e s
+      | inr1 e => Vis e (fun x => Ret (s, x))
+      end.
+
+  Definition into_reader {R} (h : R -> E ~> itree F) :
+    R -> E +' F ~> itree F :=
+    fun r _ e =>
+      match e with
+      | inl1 e => h r _ e
+      | inr1 e => ITree.liftE e
+      end.
+
+  Definition into_writer {W} (Monoid_W : Monoid W)
+             (h : E ~> writerT W (itree F))
+    : E +' F ~> writerT W (itree F) :=
+    fun _ e =>
+      match e with
+      | inl1 e => h _ e
+      | inr1 e => Vis e (fun x => Ret (monoid_unit Monoid_W, x))
+      end.
+
+  (* todo(gmm): is the a corresponding definition for `eff_hom_p`? *)
+
+End into.
