theories/Interp/Handler.v
@@ -1,0 +1,118 @@
+(** Effects [E, F : Type -> Type] and itree [E ~> itree F] form a
+    category. *)
+
+(* begin hide *)
+From ITree Require Import
+     Basics.Basics
+     Core.ITree
+     Indexed.Sum
+     Interp.Interp.
+
+Import ITree.Basics.Basics.Monads.
+Import ITreeNotations.
+
+Open Scope itree_scope.
+(* end hide *)
+
+(* Morphism Category -------------------------------------------------------- *)
+
+Definition eh_cmp {A B C} (g : B ~> itree C) (f : A ~> itree B) :
+  A ~> itree C :=
+  fun _ e => interp g _ (f _ e).
+
+Definition eh_id {A} : A ~> itree A := @ITree.liftE A.
+
+Definition eh_par {A B C D} (f : A ~> itree B) (g : C ~> itree D)
+: (A +' C) ~> itree (B +' D) :=
+  fun _ e =>
+    match e with
+    | inl1 e1 => translate (@inl1 _ _) (f _ e1)
+    | inr1 e2 => translate (@inr1 _ _) (g _ e2)
+    end.
+
+Definition eh_both {A B C} (f : A ~> itree B) (g : C ~> itree B)
+: (A +' C) ~> itree B :=
+  fun _ e =>
+    match e with
+    | inl1 e1 => f _ e1
+    | inr1 e2 => g _ e2
+    end.
+
+Definition eh_lift {A B} (m : A ~> B)  : A ~> itree B :=
+  fun _ e => ITree.liftE (m _ e).
+
+Definition eh_inl {A B} : A ~> itree (A +' B) :=
+  eh_lift (fun _ e => inl1 e).
+
+Definition eh_inr {A B} : B ~> itree (A +' B) :=
+  eh_lift (fun _ e => inr1 e).
+
+Definition eh_swap {A B} : A +' B ~> itree (B +' A) :=
+  eh_lift Sum1.swap.
+
+Definition eh_elim_empty {A} : emptyE ~> itree A :=
+  eh_lift Sum1.elim_emptyE.
+
+Definition eh_empty_left {B} : emptyE +' B ~> itree B :=
+  eh_lift Sum1.emptyE_left.
+
+Definition eh_empty_right {A} : A +' emptyE ~> itree A :=
+  eh_lift Sum1.emptyE_right.
+
+(* SAZ: do we need the assoc2 too -- add to Sum.v ? *)
+Definition eh_assoc {A B C} : (A +' (B +' C)) ~> itree ((A +' B) +' C) :=
+  eh_lift Sum1.assoc.
+
+
+
+(*
+
+
+
+(*  ------------------------------------------------------------------------- *)
+
+A Monad Transformer MT is given by:
+  MT : (type -> type) -> (type -> type)
+  lift : `{Monad m} {a}, m a -> MT m a
+
+such that:
+  Monad (MT m)
+
+  lift o return = return
+  lift o (bind t1 k) =
+
+EXAMPLE:
+   stateT S m a :=    S -> m (S * a)
+   lift : m `{Monad m} {a}, fun (c: m a) (s:S) => y <- c ;; ret (s, y)
+
+operations
+  get : m `{Monad m} stateT S m S := fun s => ret_m (s, s)
+  put : m `{Monad m}, S -> stateT S m unit := fun s' => fun s => ret_m (s', tt)
+
+(* category *)
+id : A ~> MT (itree A)
+compose : (B ~> MT2 (itree C)) ~> (A ~> MT1 (itree B)) -> (A ~> (MT2 o MT1) (itree C))
+
+(* co-cartesian *)
+par  : (A ~> MT1 (itree B)) -> (C ~> MT2 (itree D)) -> (A + C ~> (MT1 ** MT2) (itree (B + D)))
+both : (A ~> MT (itree B)) -> (C ~> (MT itree B)) -> (A + C ~> MT (itree B))
+
+swap : (A ~> MT1 (itree B)) -> (C ~> MT2 (itree D)) -> (A + C ~> (MT2 ** MT1) (itree (D + B)))
+
+
+left : A ~> MT (itree (A + B))
+right : B ~> MT (itree (A + B))
+
+left : (A ~> MT (itree B)) -> (A ~> MT (itree (B + C)))
+right : (C ~> MT (itree D)) -> (C ~> MT (itree (A + D)))
+
+(*  ------------------------------------------------------------------------- *)
+Algebraic effects handlers
+
+Definition sig (E:Type -> Type) m `{Monad m} := forall X, E X -> m x
+
+
+
+
+
+*)
