theories/Interp/HandlerFacts.v
@@ -1,0 +1,132 @@
+
+(* begin hide *)
+From Coq Require Import
+     Setoid
+     Morphisms
+     RelationClasses.
+
+From Paco Require Import paco.
+
+From ITree Require Import
+     Basics.Basics
+     Core.ITree
+     Eq.UpToTaus
+     Indexed.Sum
+     Interp.Interp
+     Interp.Handler
+     Interp.TranslateFacts
+     Interp.MorphismsFacts.
+
+Import ITree.Basics.Basics.Monads.
+Import ITreeNotations.
+
+Open Scope itree_scope.
+(* end hide *)
+
+(* Morphism Category -------------------------------------------------------- *)
+
+
+
+Lemma eh_cmp_id_left_strong :
+  forall A R (t : itree A R), interp eh_id R t ≈ t.
+Proof.
+  intros A R.
+  intros t.
+  pupto2_init; revert t; pcofix CIH; intros t.
+  pfold; pupto2_init; revert t; pcofix CIH'; intros.
+  rewrite unfold_interp. unfold interp_u.
+  destruct (observe t); cbn; eauto.
+  - pfold. econstructor. auto.
+  - unfold eh_id, ITree.liftE. rewrite vis_bind.
+    pfold; do 2 constructor.
+    left; rewrite ret_bind; auto.
+Qed.
+
+
+Lemma eh_cmp_id_left :
+  forall A B (f : A ~> itree B), eh_cmp eh_id f ≡ f.
+Proof.
+  intros A B f X e.
+  unfold eh_cmp. apply eh_cmp_id_left_strong.
+Qed.
+
+
+Lemma eh_cmp_id_right :
+  forall A B (f : A ~> itree B), eh_cmp f eh_id ≡ f.
+Proof.
+  intros B A f X e.
+  unfold eh_cmp.
+  unfold eh_id. unfold ITree.liftE.
+  rewrite unfold_interp. unfold interp_u.
+  cbn. setoid_rewrite tau_eutt. setoid_rewrite interp_ret. rewrite bind_ret.
+  reflexivity.
+Qed.
+
+Lemma eh_both_left_right_id : forall A B X e,  eh_both eh_inl eh_inr X e = (@eh_id (A +' B)) X e.
+Proof.
+  intros A B X e.
+  unfold eh_both.
+  unfold eh_id. unfold ITree.liftE.
+  destruct e.
+  - unfold eh_inl. reflexivity.
+  - unfold eh_inr. reflexivity.
+Qed.
+
+Lemma eh_cmp_assoc : forall A B C D (h : C ~> itree D) (g : B ~> itree C) (f : A ~> itree B),
+    eh_cmp h (eh_cmp g f) ≡ (eh_cmp (eh_cmp h g) f).
+Proof.
+  intros A B C D h g f X e.
+  unfold eh_cmp. rewrite interp_interp. reflexivity.
+Qed.
+
+Lemma eh_par_id : forall A B, eh_par eh_id eh_id ≡ (@eh_id (A +' B)).
+Proof.
+  intros A B X e.
+  unfold eh_par.
+  unfold eh_id.
+  destruct e.
+  - unfold ITree.liftE.
+    rewrite translate_vis.
+    assert (pointwise_relation X (@eq_itree (A +' B) _ _ eq) (fun x : X => translate (inl1 (E2:=B)) (Ret x)) (fun x : X => Ret x)).
+    { intros x. rewrite translate_ret. reflexivity. }
+    rewrite H. reflexivity.
+  - unfold ITree.liftE.
+    rewrite translate_vis.
+    assert (pointwise_relation X (@eq_itree (A +' B) _ _ eq) (fun x : X => translate (inr1 (E2:=B)) (Ret x)) (fun x : X => Ret x)).
+    { intros x. rewrite translate_ret. reflexivity. }
+    rewrite H. reflexivity.
+Qed.
+
+
+Lemma eh_swap_swap_id : forall A B, eh_cmp eh_swap eh_swap ≡ (eh_id : (A +' B) ~> itree (A +' B)).
+Proof.
+  intros A B X e.
+  unfold eh_cmp. unfold eh_swap. unfold eh_lift.
+  rewrite interp_liftE.
+  setoid_rewrite tau_eutt. rewrite bind_ret.
+  destruct e; simpl; reflexivity.
+Qed.
+
+Lemma eh_empty_unit_l : forall A, eh_cmp eh_empty_right eh_inl ≡ (eh_id : A ~> itree A).
+Proof.
+  intros A X e.
+  unfold eh_cmp.
+  unfold eh_empty_right.
+  unfold eh_inl.
+  unfold eh_lift.
+  rewrite interp_liftE.
+  setoid_rewrite tau_eutt. rewrite bind_ret.
+  simpl. unfold Sum1.idE. reflexivity.
+Qed.
+
+Lemma eh_empty_unit_r : forall A, eh_cmp eh_empty_left eh_inr ≡ (eh_id : A ~> itree A).
+Proof.
+  intros A X e.
+  unfold eh_cmp.
+  unfold eh_empty_left.
+  unfold eh_inr.
+  unfold eh_lift.
+  rewrite interp_liftE.
+  setoid_rewrite tau_eutt. rewrite bind_ret.
+  simpl. unfold Sum1.idE. reflexivity.
+Qed.
